

{\bf Numerical solution}\\

\begin{eqnarray}\label{final_eq}
\left[ \begin{array}{cc}
\tenss{K}_{hh} & \tenss{K}_{hT} \\
\tenss{K}_{Th} & \tenss{K}_{TT}
\end{array} \right]
\left\{ \begin{array}{c}
\tenss{r}_h \\
\tenss{r}_{T}
\end{array} \right\} + 
\left[ \begin{array}{cc}
\tenss{C}_{hh} & \tenss{C}_{hT} \\
\tenss{C}_{Th} & \tenss{C}_{TT}
\end{array} \right]
\left\{ \begin{array}{c}
\dot{\tenss{r}}_h \\
\dot{\tenss{r}}_{T}
\end{array} \right\} = 
\left\{ \begin{array}{c}
\tenss{q}_{h} \\
\tenss{q}_{T}
\end{array} \right\},
\end{eqnarray}
where
\begin{eqnarray}
\tenss{K}_{hh} = \int_{\Omega} \tenss{B}^T k_{hh} \tenss{B}{\rm d}\Omega,
\qquad \tenss{K}_{hT} = \int_{\Omega} \tenss{B}^T k_{hT} \tenss{B}{\rm d}\Omega,
\end{eqnarray}
\begin{eqnarray}
\tenss{K}_{Th} = \int_{\Omega} \tenss{B}^T k_{Th} \tenss{B}{\rm d}\Omega,
\qquad \tenss{K}_{TT} = \int_{\Omega} \tenss{B}^T k_{TT} \tenss{B}{\rm d}\Omega,
\end{eqnarray}
\begin{eqnarray}
\tenss{C}_{hh} = \int_{\Omega} \tenss{N}^T c_{hh}  \tenss{N} {\rm d}\Omega,\qquad
\tenss{C}_{hT} = \int_{\Omega} \tenss{N}^T c_{hT}  \tenss{N} {\rm d}\Omega,\qquad
\end{eqnarray}
\begin{eqnarray}
\tenss{C}_{Th} = \int_{\Omega} \tenss{N}^T c_{Th}  \tenss{N} {\rm d}\Omega,\qquad
\tenss{C}_{TT} = \int_{\Omega} \tenss{N}^T c_{TT}  \tenss{N} {\rm d}\Omega,\qquad
\end{eqnarray}
\begin{eqnarray}
\tenss{q}_h = \int_{\Gamma_2} \tenss{N}^T  \overline{q}^{h}{\rm d}\Gamma,\qquad
\tenss{q}_T = \int_{\Gamma_2} \tenss{N}^T  \overline{q}_{T}{\rm d}\Gamma,\qquad
\end{eqnarray}

where
\begin{eqnarray}
 k_{hh} = ,
\qquad k_{hT} = ,
\end{eqnarray}
\begin{eqnarray}
 k_{Th} = ,
\qquad k_{TT} = ,
\end{eqnarray}
\begin{eqnarray}
 c_{hh} = ,
\qquad c_{hT} = ,
\end{eqnarray}
\begin{eqnarray}
 c_{Th} = ,
\qquad c_{TT} = ,
\end{eqnarray}
